theories/typing/uninit.v
@@ -1,49 +1,44 @@
 Require Import FunctionalExtensionality Equality.
 From lrust.typing Require Export type.
-From lrust.typing Require Import mod_ty array product.
 Set Default Proof Using "Type".
 
 Section uninit.
   Context `{!typeG Σ}.
 
-  Program Definition uninit1: type () :=
-    {| pt_size := 1;  pt_own _ _ vl := ⌜∃v, vl = [v]⌝; |}%I.
-  Next Obligation. by iIntros "*[%->]". Qed.
-
-  Definition uninit (n: nat) : type () := <{unique}> [uninit1; n].
+  Program Definition uninit n : type unit := {|
+    ty_size := n;  ty_lfts := [];  ty_E := [];
+    ty_own _ _ _ vl := ⌜length vl = n⌝;  ty_shr _ _ _ _ _ := True;
+  |}%I.
+  Next Obligation. by iIntros. Qed. Next Obligation. by iIntros. Qed.
+  Next Obligation. by iIntros. Qed. Next Obligation. by iIntros. Qed.
+  Next Obligation. iIntros. iApply step_fupdN_intro; [done|]. by iFrame. Qed.
+  Next Obligation.
+    iIntros. iApply step_fupdN_full_intro. iIntros "!>!>". iExists [], 1%Qp.
+    iSplit; [|simpl; by iFrame]. iPureIntro. apply proph_dep_unique.
+  Qed.
+  Next Obligation.
+    iIntros. iApply step_fupdN_full_intro. iIntros "!>!>!>!>". iExists [], 1%Qp.
+    iSplit; [|simpl; by iFrame]. iPureIntro. apply proph_dep_unique.
+  Qed.
 
 End uninit.
 
 Notation "↯" := uninit : lrust_type_scope.
+Notation unit_ty := (uninit 0).
+Notation "()" := unit_ty : lrust_type_scope.
 
 Section typing.
   Context `{!typeG Σ}.
 
-  Global Instance uninit1_send: Send uninit1. Proof. done. Qed.
-  Global Instance uninit1_sync: Sync uninit1. Proof. done. Qed.
+  Global Instance uninit_send n : Send (uninit n). Proof. done. Qed.
+  Global Instance uninit_sync n : Sync (uninit n). Proof. done. Qed.
 
-  Lemma uninit_own n vπ d tid vl : (↯ n).(ty_own) vπ d tid vl ⊣⊢ ⌜length vl = n⌝.
+  Global Instance unit_ty_copy: Copy ().
   Proof.
-    rewrite mod_ty_own. move: vl. elim: n=> [|n IH] vl.
-    - by rewrite mod_ty_own length_zero_iff_nil.
-    - rewrite mod_ty_own -/hrepeat -/xprod_ty. iSplit.
-      + iDestruct 1 as (??->[?[_[?->]]]) "H /=". rewrite IH. by iDestruct "H" as %->.
-      + case vl=>/= [|v vl']; iIntros ([=]). iExists [v], vl'. rewrite IH.
-        iPureIntro. split; [done|]. split; [|done]. exists (). split; by [|exists v].
-  Qed.
-
-  Lemma uninit_0_unit: (↯ 0 ≡ ())%T.
-  Proof.
-    split=>// *; [rewrite !mod_ty_own|rewrite !mod_ty_shr];
-    by rewrite compose_assoc semi_iso.
-  Qed.
-
-  Lemma uninit_plus_prod E L m n :
-    eqtype E L unique unique (↯ (m + n)) (↯ m * ↯ n).
-  Proof.
-    eapply eqtype_eq. { eapply eqtype_trans; [apply mod_ty_outin, _|].
-    eapply eqtype_trans; [apply array_plus_prod|].
-    apply prod_eqtype; apply mod_ty_inout, _. } { done. } { done. }
+    split; [apply _|]=> *. iIntros "_ _ Na $ !> /=". iExists 1%Qp, [].
+    rewrite heap_mapsto_vec_nil.
+    iDestruct (na_own_acc with "Na") as "[$ ToNa]"; [solve_ndisj|].
+    do 2 (iSplit; [done|]). iIntros "Na". by iDestruct ("ToNa" with "Na") as "$".
   Qed.
 
 End typing.
